theories/L6_PCPS/cps_proto_metacoq.v
@@ -3,35 +3,12 @@ Import ListNotations.
 
 From MetaCoq Require Import Template.All.
 
-From CertiCoq.L6 Require Import PrototypeGenFrame.
+From CertiCoq.L6 Require Import PrototypeGenFrame cps.
 
-Unset Strict Unquote Universe Mode.
-
-Inductive var      := mk_var : positive -> var.
-Inductive fun_tag  := mk_fun_tag : positive -> fun_tag.
-Inductive ctor_tag := mk_ctor_tag : positive -> ctor_tag.
-Inductive prim     := mk_prim : positive -> prim.
-
-Definition un_var := fun '(mk_var x) => x.
-Definition un_fun_tag := fun '(mk_fun_tag x) => x.
-Definition un_ctor_tag := fun '(mk_ctor_tag x) => x.
-Definition un_prim := fun '(mk_prim x) => x.
-
-Inductive exp : Type :=
-| Econstr (x : var) (c : ctor_tag) (ys : list var) (e : exp)
-| Ecase (x : var) (ces : list (ctor_tag * exp))
-| Eproj (x : var) (c : ctor_tag) (n : N) (y : var) (e : exp)
-| Eletapp (x : var) (f : var) (ft : fun_tag) (ys : list var) (e : exp)
-| Efun (fds : list fundef) (e : exp)
-| Eapp (f : var) (ft : fun_tag) (xs : list var)
-| Eprim (x : var) (p : prim) (ys : list var) (e : exp)
-| Ehalt (x : var)
-with fundef : Type :=
-| Ffun (f : var) (ft : fun_tag) (xs : list var) (e : exp).
-
-(* Takes a while to save aux_data *)
 Run TemplateProgram (mk_Frame_ops
   "exp" exp [var; fun_tag; ctor_tag; prim; N; list var]).
+Print exp_univ.
+Print exp_univD.
 
 Instance Frame_exp : Frame exp_univ := exp_Frame_ops.
 Instance AuxData_exp : AuxData exp_univ := exp_aux_data.
